Progress

Gadgets.v
@@ -3,37 +3,50 @@ From STLCZK Require Import Stlc.
 
 Require Import Coqprime.elliptic.ZEll.
 Require Import Coq.Numbers.BinNums.
+Require Import Coqprime.elliptic.GZnZ.
+Require Import Coq.ZArith.Znumtheory.
+Require Import Coq.ZArith.BinIntDef.
+Import Z.
+Require Import Coq.ZArith.BinInt.
 
 Module Gadgets.
-  Import Stlc_Fp.
-  
+
+  Include Stlc_Fp.
+
   Definition X : atom := fresh nil.
   Definition Y : atom := fresh (X :: nil).
   
   (** Notation on Stlc_Ott *)
   
   Coercion tm_var_f: expvar >-> exp.
-  Coercion const_field: Fp >-> constant.
   Coercion tm_constant: constant >-> exp.
   
   Declare Custom Entry stlc_ty.
   Declare Custom Entry stlc.
+  Notation "'fp' n" := (const_field n) (in custom stlc at level 0).
+  Notation "'F0'" := (const_field fp_zero) (in custom stlc at level 0).
+  Notation "'F1'" := (const_field fp_one) (in custom stlc at level 0).
+  Notation "'true'" := (const_true) (in custom stlc at level 0).
+  Notation "'false'" := (const_false) (in custom stlc at level 0).
   Notation "<{ e }>" := e (e custom stlc at level 99).
   Notation "<{{ e }}>" := e (e custom stlc_ty at level 99).
   Notation "( x )" := x (in custom stlc, x at level 99).
   Notation "( x )" := x (in custom stlc_ty, x at level 99).
   Notation "x" := x (in custom stlc at level 0, x constr at level 0).
   Notation "x" := x (in custom stlc_ty at level 0, x constr at level 0).
-  Notation "S -> T" := (ty_arrow S T) (in custom stlc_ty at level 50, right associativity).
+  
   Notation "x y" := (tm_app x y) (in custom stlc at level 1, left associativity).
   Notation "\_ : t , y" :=
     (tm_abs t y) (in custom stlc at level 90,
                      t custom stlc_ty at level 99,
                      y custom stlc at level 99,
                      left associativity).
-  Notation "# n" := (tm_var_b n) (in custom stlc at level 1).
+  Notation "# n" := (tm_var_b n%nat) (in custom stlc at level 1).
   Notation "{ x }" := x (in custom stlc at level 1, x constr).
 
+  Notation "S -> T" := (ty_arrow S T) (in custom stlc_ty at level 0, right associativity).
+  Notation "Gamma '|-' t '::' T" := (typing Gamma t T) (in custom stlc_ty at level 40, t custom stlc, T custom stlc_ty at level 1).
+                                                                       
   Notation "'Field'" := ty_field (in custom stlc_ty at level 0).
   Notation "'Bool'" := ty_bool (in custom stlc_ty at level 0).
 
@@ -46,13 +59,13 @@ Module Gadgets.
                                                 left associativity).
   Notation "x / y" := (tm_binop x op_div y) (in custom stlc at level 1,
                                                 left associativity).
-  Notation "x && y" := (tm_binop x op_and y) (in custom stlc at level 2,
+  Notation "x && y" := (tm_binop x op_and y) (in custom stlc at level 4,
                                                  left associativity).
-  Notation "x || y" := (tm_binop x op_or y) (in custom stlc at level 2,
+  Notation "x || y" := (tm_binop x op_or y) (in custom stlc at level 4,
                                                left associativity).
-  Notation "x == y" := (tm_eq x y) (in custom stlc at level 1,
+  Notation "x == y" := (tm_eq x y) (in custom stlc at level 3,
                                        left associativity).
-  Notation "! x " := (tm_not x) (in custom stlc at level 1).
+  Notation "! x " := (tm_not x) (in custom stlc at level 3).
 
   Notation "'if' x 'then' y 'else' z" :=
     (tm_ifthenelse x y z) (in custom stlc at level 89,
@@ -76,42 +89,23 @@ Module Gadgets.
 
   (** Example 1: Division *)
   Definition div :=
-    <{ \_: Field, ({const_field fp_one} / #0) }>.
+    <{ \_: Field, (F1 / #0) }>.
 
-  Definition div_applied(c: Fp) :=
-    <{ div ({const_field c}) }>.
-  Definition foo(c: Fp) :=
-    match div_applied c with
-    | tm_app ((tm_abs _ e1)) v => true
-    | _ => false
-    end.
-
-  Compute foo fp_one.
-  (** step (tm_app  ( (tm_abs T e1) )  v2)  (open_exp_wrt_exp  e1   v2 ) *)
-  
-  Print div_applied. 
   Definition div_check :=
     <{ \_: Field,
            (\_: Field,
-                #0 * #1 == ({const_field fp_one}))
+                (#0 * #1) == F1)
      }>.
 
-  Definition circuit_equiv1(c: exp) (c': exp): Prop :=
-    forall (n: Fp), exists (ans: Fp),
-        typing nil c (ty_arrow ty_field ty_field) /\
-        typing nil c' (ty_arrow ty_field (ty_arrow ty_field ty_bool)) ->
-        (<{ c' n ans }> -->* const_true <->
-        <{ c n }> -->* ans).
-   
-  Notation "a '~' b" := (circuit_equiv1 a b) (at level 50).
 
-  Definition circuit_equiv2(c: exp) (c': exp): Prop :=
-    forall (n: Fp), forall (ans: Fp),
-        <{ c' n ans }> -->* const_true <->
-        <{ c n }> -->* ans.
+  Definition circuit_equiv(c: exp) (c': exp): Prop :=
+    forall (n: Fp), forall (w: Fp),
+        <{{ nil |- c :: Field -> Field }}> ->
+        <{{ nil |- c' :: Field -> Field -> Bool }}> ->
+        (<{ c' (fp n) (fp w) }> -->* <{ true }> <->
+        <{ c (fp n) }> -->* <{ fp w }>).
    
-  Notation "a '~~' b" := (circuit_equiv2 a b) (at level 50).
-
+  Notation "a '~~' b" := (circuit_equiv a b) (at level 50).
   
   Ltac invert H := inversion H; subst; clear H.
   Ltac invert_log_solved H g := 
@@ -121,69 +115,125 @@ Module Gadgets.
     repeat match goal with
            | [ H: <{ (open_exp_wrt_exp _ _) }> -->* _ |- _ ] => idtac "cbn"; cbn in H
            | [ H: <{ (open_exp_wrt_exp _ _) _ }> -->* _ |- _ ] => idtac "cbn"; cbn in H        
-           | [ H: step ?a ?b |- ?g ] => idtac "Inverting" a "-->" b "for" g; invert_log_solved H g
-           | [ H: ?a -->* ?b |- _ ] => idtac "Big-step" a "-->*" b; inversion H; subst; clear H
+           | [ H: step ?a ?b |- ?g ] => invert_log_solved H g
+           | [ H: ?a -->* ?b |- _ ] => inversion H; subst; clear H
            end.
-  
+
+  Lemma neq_const: forall a b, <{ fp a }> <> <{ fp b }> -> a <> b.
+  Proof.
+    intros.
+    destruct (eq_fp a b).
+    - subst. contradiction.
+    - assumption.
+  Qed.
+
+  Require Import Coq.setoid_ring.Field_theory.
+  Require Import Coq.ZArith.BinInt.
+  Print ring_theory.
+
+  Lemma fp_mul_div_n0 : forall n w, n <> fp_zero ->
+                             pkdiv (pkmul w n) n = w.
+  Proof.
+    intros.
+    pose proof (pKfth p_prime) as FT.
+    invert FT.
+    rewrite Fdiv_def.
+    invert F_R.
+    rewrite <- Rmul_assoc.
+    apply Finv_l in H.
+    replace (pkmul n (pkinv n)) with (pkmul (pkinv n) n) by (apply Rmul_comm).
+    rewrite H.
+    rewrite <- Rmul_comm.
+    rewrite Rmul_1_l.
+    reflexivity.
+  Qed.
+
+  Lemma neq_stlc_fp: forall n w, <{ fp n }> <> <{ fp w }> <-> n <> w.
+  Proof.
+    intro n.
+    destruct n as (n', n_mod).
+    induction n'; split; intros.
+    - intro. invert H0; contradiction.
+    - intro. invert H0; contradiction.
+    - intro. invert H0; contradiction.
+    - intro. invert H0; contradiction.
+    - intro. invert H0; contradiction.
+    - intro. invert H0; contradiction.
+  Qed.
+
   (** This is not complete over all possible witnesses, but still passes *)
-  Theorem div_gadget_equiv_1_noncomplete: div ~ div_check.
+  Theorem div_gadget_equiv: div ~~ div_check.
   Proof.
-    unfold circuit_equiv1, div, div_check.
-    intros.
-    destruct n as (n', n_mod) eqn:N.
-    induction n'.
-    - exists fp_zero.
-      intros [H_tyc H_tyc'].
-      split; intro H; solve_stlc.
-      unfold fp_zero, pkO, GZnZ.zero in *.
-      apply eq_fp in H5.
-      cbn in H5.
-      intro H.
-      solve_stlc.
-
-      intro H. solve_stlc.
-      solve_stlc.
-      invert H.
-      invert H0.
-      invert H5.
-      invert H6.
-      invert H7.
-
-      solve_stlc.
-      invert H1.
-      invert H.
-      solve_stlc.
-
-      invert H10.
-      
-      cbn in H1.
-      intro H; solve_stlc.
-  Qed.
-
-  
-  Theorem div_gadget_equiv_2_complete: div ~~ div_check.
-  Proof.
-    unfold circuit_equiv2, div, div_check.
-    intros.    
+    unfold circuit_equiv, div, div_check.
+    intros n w Hty Hty'.
     split; intro H; solve_stlc.
-  Qed.
-  
-  (** This is complete over all possible witnesses, 
-      how to make this accepted but the above not ? *)
-  Theorem div_gadget_equiv_1_complete: div ~ div_check.
-  Proof.
-    unfold circuit_equiv1, div, div_check.
-    intros.
-    destruct n as (n', Hmod_n) eqn:F.
-    induction n'.
-    - exists fp_zero.
-      split; intro H; solve_stlc.
-    - exists (pkdiv fp_one n).
-      split; intro H; solve_stlc.
-    - exists (pkdiv (pkopp fp_one) n).
-      split; intro H; solve_stlc.
-  Qed.
-
+    - econstructor.
+      eapply step_beta; repeat constructor.
+      + econstructor. intros. cbn.
+        constructor. constructor. constructor.
+      + cbn.
+        destruct (eq_fp n fp_zero).
+        * subst.
+          unfold pkmul in H9.
+          invert H9.
+          rewrite Zmult_comm in H0.
+          simpl in *.
+          pose proof (p_prime).
+          invert H.
+          rewrite Z.mod_0_l in H0.
+          rewrite Z.mod_1_l in H0.
+          invert H0.
+          assumption.
+          intro.
+          rewrite H in H1.
+          invert H1.
+        * econstructor.
+          eapply step_div_const.
+          intro.
+          invert H.
+          contradiction.
+          rewrite fp_mul_div_n0.         
+          eapply multi_refl.
+          assumption.
+    - econstructor.      
+      eapply step_app_1. repeat constructor.      
+      eapply step_beta. repeat constructor.
+      econstructor.
+      intros.
+      cbn.
+      econstructor.
+      intros.
+      cbn.
+      repeat constructor.
+      repeat constructor.
+      cbn.
+      econstructor.
+    
+      eapply step_beta; repeat constructor.
+      econstructor.
+      intros.
+      cbn.      
+      repeat constructor.
+      cbn.
+      econstructor.
+      eapply step_eq_cog_1. repeat constructor.
+      eapply step_mul_const.
+      pose proof (pKfth p_prime) as FT.
+      invert FT.
+      invert F_R.
+      rewrite Fdiv_def.
+      rewrite <- Rmul_assoc.
+      rewrite neq_stlc_fp in H5.
+      apply Finv_l in H5.
+      rewrite H5.
+      rewrite Rmul_1_l.
+      econstructor.
+      eapply step_eq_refl.
+      apply multi_refl.
+      Unshelve.
+      (** Some atoms are left as holes! How to specify? *)
+  Admitted.
+ 
   Fixpoint constant_to_boolnat(c: constant) : Fp :=
     match c with
     | const_true => fp_one
@@ -223,4 +273,8 @@ Module Gadgets.
     intros; split; intro H; solve.
   Qed.
 
+  repeat match goal with
+               | [ _ |- _ -->* _ ] => econstructor
+               | [ _ |- step <{ (\_: ?F, _) _ }>  _ => idtac "beta"; eapply step_beta
+               | [ _
 End Gadgets.     
